mem/Mem0.v
@@ -1,9 +1,9 @@
-Require Import Coqlib.
+Require Import Coqlib Algebra.
 Require Import ITreelib.
 Require Import ImpPrelude.
 Require Import STS.
 Require Import Behavior.
-Require Import Mod ModSem.
+Require Import Mod ModSem LSimModSem.
 Require Import Skeleton.
 
 Set Implicit Arguments.
@@ -85,6 +85,36 @@ Section PROOF.
     |}
   .
 
+  Lemma equiv_load_mem: forall sk0 sk1, Sk.wf sk0 -> sk0 ≡ sk1 -> Mem.load_mem sk0 = Mem.load_mem sk1.
+  Proof.
+    ii. r in H0. unfold Mem.load_mem. f_equiv. extensionalities b ofs.
+    uo. des_ifs_safe; ss. destruct b; ss. clarify.
+    destruct (alist_find s sk0) eqn:T.
+    - erewrite alist_permutation_find in T; et. des_ifs.
+    - erewrite alist_permutation_find in T; et. des_ifs.
+  Qed.
+
+  Definition mem_extends (m0 m1: Mem.t): Prop :=
+    <<BLK: forall b, m0.(Mem.cnts) (inl b) = m1.(Mem.cnts) (inl b)>> /\
+    <<NAME: forall fn ofs v, m0.(Mem.cnts) (inr fn) ofs = Some v -> m1.(Mem.cnts) (inr fn) ofs = Some v>> /\
+    (* <<CNTS: forall b ofs v, m0.(Mem.cnts) b ofs = Some v -> m1.(Mem.cnts) b ofs = Some v>> /\ *)
+    <<NB: m0.(Mem.nb) = m1.(Mem.nb)>>
+  .
+
+  Lemma extends_valid_ptr m0 m1: mem_extends m0 m1 ->
+                                 forall b ofs, Mem.valid_ptr m0 b ofs = true -> Mem.valid_ptr m1 b ofs = true.
+  Proof.
+    ii; ss. rr in H. des. unfold Mem.valid_ptr in *. unfold is_some in *. des_ifs.
+    exfalso. destruct b; ss; et.
+    - erewrite BLK in *; ss. congruence.
+    - eapply NAME in Heq0; ss. congruence.
+  Qed.
+
+  Ltac my_steps :=
+    repeat (esplits; my_red_both;
+            try (guclo sim_itree_indC_spec; first [apply sim_itree_indC_choose_tgt|apply sim_itree_indC_take_src|econs]; et);
+            i; des; ss; subst; et).
+
   Program Definition Mem: Mod.t := {|
     Mod.get_modsem := MemSem;
     Mod.sk := Sk.unit;
@@ -92,10 +122,229 @@ Section PROOF.
   .
   Next Obligation.
     ii. r in EQV. unfold MemSem. ss. f_equiv.
-    f_equiv. unfold Mem.load_mem. f_equiv. extensionalities b ofs.
-    uo. des_ifs_safe; ss. destruct b; ss. clarify.
-    destruct (alist_find s sk0) eqn:T.
-    - erewrite alist_permutation_find in T; et. des_ifs.
-    - erewrite alist_permutation_find in T; et. des_ifs.
+    f_equiv. erewrite equiv_load_mem; ss.
   Qed.
+  Next Obligation.
+    eapply ModSemPair.adequacy. ss.
+    econs.
+    { instantiate (1:=top2). ss. }
+    2: { instantiate (2:=unit).
+         instantiate (1:=fun _ '(st_src, st_tgt) =>
+                           exists m0 m1, st_tgt = Any.upcast m0 /\ st_src = Any.upcast m1 /\ mem_extends m1 m0).
+         ss. esplits; ss; et.
+         r. esplits; ss. i. uo. des_ifs_safe.
+         rr in EQV. des. rr in EQV. unfold oplus, Sk.add in *. ss. rr in WF.
+         erewrite alist_permutation_find.
+         2: { et. }
+         2: { sym; et. }
+         erewrite alist_find_app; et. ss.
+    }
+    ss. ii. des; ss; clarify.
+    {
+      esplits; ss; et. ii. des; subst.
+      rr in SIMMRS1. des.
+      eapply sim_itree_fsubset with []; ss.
+      unfold cfunU, allocF.
+      ginit. my_steps.
+      destruct (Any.downcast y) eqn:T.
+      2: { cbn. unfold triggerUB. my_steps. }
+      my_steps. des_ifs; my_steps; unfold triggerUB; my_steps.
+      destruct v; my_steps; des_ifs; my_steps; unfold triggerUB; my_steps.
+      rr. esplits; ss; et.
+      2: { rewrite NB; ss. }
+      rr. ss. esplits; try lia.
+      - ii. rewrite NB in *. unfold update in *. des_ifs; ss; et.
+      - ii. rewrite NB in *. unfold update in *. des_ifs; ss; et.
+    }
+    {
+      esplits; ss; et. ii. des; subst.
+      rr in SIMMRS1. des.
+      eapply sim_itree_fsubset with []; ss.
+      unfold cfunU, freeF.
+      ginit. my_steps.
+      destruct (Any.downcast y) eqn:T.
+      2: { cbn. unfold triggerUB. my_steps. }
+      my_steps. des_ifs; my_steps; unfold triggerUB; my_steps.
+      destruct v; my_steps; des_ifs; my_steps; unfold triggerUB; my_steps.
+      destruct blk; my_steps; des_ifs; my_steps; unfold triggerUB; my_steps.
+      destruct (Mem.free m1 n ofs) eqn:U.
+      2: { cbn. unfold triggerUB. my_steps. }
+      my_steps.
+      unfold Mem.free in *. des_ifs_safe. rewrite <- BLK. des_ifs. my_steps.
+      rr. esplits; ss; et.
+      rr. ss. esplits; try lia.
+      - ii. unfold update in *. des_ifs; ss; et.
+      - ii. unfold update in *. des_ifs; ss; et.
+    }
+    {
+      esplits; ss; et. ii. des; subst.
+      rr in SIMMRS1. des.
+      eapply sim_itree_fsubset with []; ss.
+      unfold cfunU, loadF.
+      ginit. my_steps.
+      destruct (Any.downcast y) eqn:T.
+      2: { cbn. unfold triggerUB. my_steps. }
+      my_steps. des_ifs; my_steps; unfold triggerUB; my_steps.
+      destruct v; my_steps; des_ifs; my_steps; unfold triggerUB; my_steps.
+      destruct (Mem.load m1 blk ofs) eqn:U.
+      2: { cbn. unfold triggerUB. my_steps. }
+      my_steps.
+      assert(V: Mem.load m0 blk ofs = Some v).
+      { destruct blk; ss; et. rewrite <- BLK; et. }
+      rewrite V; ss. my_steps.
+      rr. esplits; ss; et.
+    }
+    {
+      esplits; ss; et. ii. des; subst.
+      rr in SIMMRS1. des.
+      eapply sim_itree_fsubset with []; ss.
+      unfold cfunU, storeF.
+      ginit. my_steps.
+      destruct (Any.downcast y) eqn:T.
+      2: { cbn. unfold triggerUB. my_steps. }
+      my_steps. des_ifs; my_steps; unfold triggerUB; my_steps.
+      destruct v; my_steps; des_ifs; my_steps; unfold triggerUB; my_steps.
+      destruct (Mem.store m1 blk ofs) eqn:U.
+      2: { cbn. unfold triggerUB. my_steps. }
+      my_steps.
+      unfold Mem.store in *. des_ifs_safe.
+      assert(U: Mem.cnts m0 blk ofs = Some v).
+      { destruct blk; ss; et. rewrite <- BLK; et. }
+      des_ifs. my_steps.
+      rr. esplits; ss; et.
+      rr. ss. esplits; try lia.
+      - ii. extensionalities ofs0. rewrite BLK; ss.
+      - ii. des_ifs; ss; et.
+    }
+    {
+      esplits; ss; eauto 10. ii. des; subst.
+      assert(W:=extends_valid_ptr SIMMRS1).
+      rr in SIMMRS1. des.
+      eapply sim_itree_fsubset with []; ss.
+      unfold cfunU, cmpF.
+      ginit. my_steps.
+      destruct (Any.downcast y) eqn:T.
+      2: { cbn. unfold triggerUB. my_steps. }
+      my_steps. des_ifs; my_steps; unfold triggerUB; my_steps.
+      destruct (vcmp m1 v v0) eqn:U.
+      2: { cbn. unfold triggerUB. my_steps. }
+      unfold vcmp in *. des_ifs; my_steps; des_ifs; my_steps; rr; esplits; ss;
+        bsimpl; des; des_sumbool; ss; subst; exploit W; et; i; try congruence.
+      - clear Heq2. exploit W; et; i; try congruence.
+      - clear Heq2. exploit W; et; i; try congruence.
+    }
+  Qed.
+  Next Obligation.
+    assert( | MemSem sk1 | = | MemSem sk0 | ).
+    { unfold bar; ss. f_equiv. unfold bar; ss. f_equiv.
+    eapply ModSemPair.adequacy. ss.
+    econs.
+    { instantiate (1:=top2). ss. }
+    2: { instantiate (2:=unit).
+         instantiate (1:=fun _ '(st_src, st_tgt) =>
+                           exists m0 m1, st_tgt = Any.upcast m0 /\ st_src = Any.upcast m1 /\ mem_extends m1 m0).
+         ss. esplits; ss; et.
+         r. esplits; ss. i. uo. des_ifs_safe.
+         rr in EQV. des. rr in EQV. unfold oplus, Sk.add in *. ss. rr in WF.
+         erewrite alist_permutation_find.
+         2: { et. }
+         2: { sym; et. }
+         erewrite alist_find_app; et. ss.
+    }
+    ss. ii. des; ss; clarify.
+    {
+      esplits; ss; et. ii. des; subst.
+      rr in SIMMRS1. des.
+      eapply sim_itree_fsubset with []; ss.
+      unfold cfunU, allocF.
+      ginit. my_steps.
+      destruct (Any.downcast y) eqn:T.
+      2: { cbn. unfold triggerUB. my_steps. }
+      my_steps. des_ifs; my_steps; unfold triggerUB; my_steps.
+      destruct v; my_steps; des_ifs; my_steps; unfold triggerUB; my_steps.
+      rr. esplits; ss; et.
+      2: { rewrite NB; ss. }
+      rr. ss. esplits; try lia.
+      - ii. rewrite NB in *. unfold update in *. des_ifs; ss; et.
+      - ii. rewrite NB in *. unfold update in *. des_ifs; ss; et.
+    }
+    {
+      esplits; ss; et. ii. des; subst.
+      rr in SIMMRS1. des.
+      eapply sim_itree_fsubset with []; ss.
+      unfold cfunU, freeF.
+      ginit. my_steps.
+      destruct (Any.downcast y) eqn:T.
+      2: { cbn. unfold triggerUB. my_steps. }
+      my_steps. des_ifs; my_steps; unfold triggerUB; my_steps.
+      destruct v; my_steps; des_ifs; my_steps; unfold triggerUB; my_steps.
+      destruct blk; my_steps; des_ifs; my_steps; unfold triggerUB; my_steps.
+      destruct (Mem.free m1 n ofs) eqn:U.
+      2: { cbn. unfold triggerUB. my_steps. }
+      my_steps.
+      unfold Mem.free in *. des_ifs_safe. rewrite <- BLK. des_ifs. my_steps.
+      rr. esplits; ss; et.
+      rr. ss. esplits; try lia.
+      - ii. unfold update in *. des_ifs; ss; et.
+      - ii. unfold update in *. des_ifs; ss; et.
+    }
+    {
+      esplits; ss; et. ii. des; subst.
+      rr in SIMMRS1. des.
+      eapply sim_itree_fsubset with []; ss.
+      unfold cfunU, loadF.
+      ginit. my_steps.
+      destruct (Any.downcast y) eqn:T.
+      2: { cbn. unfold triggerUB. my_steps. }
+      my_steps. des_ifs; my_steps; unfold triggerUB; my_steps.
+      destruct v; my_steps; des_ifs; my_steps; unfold triggerUB; my_steps.
+      destruct (Mem.load m1 blk ofs) eqn:U.
+      2: { cbn. unfold triggerUB. my_steps. }
+      my_steps.
+      assert(V: Mem.load m0 blk ofs = Some v).
+      { destruct blk; ss; et. rewrite <- BLK; et. }
+      rewrite V; ss. my_steps.
+      rr. esplits; ss; et.
+    }
+    {
+      esplits; ss; et. ii. des; subst.
+      rr in SIMMRS1. des.
+      eapply sim_itree_fsubset with []; ss.
+      unfold cfunU, storeF.
+      ginit. my_steps.
+      destruct (Any.downcast y) eqn:T.
+      2: { cbn. unfold triggerUB. my_steps. }
+      my_steps. des_ifs; my_steps; unfold triggerUB; my_steps.
+      destruct v; my_steps; des_ifs; my_steps; unfold triggerUB; my_steps.
+      destruct (Mem.store m1 blk ofs) eqn:U.
+      2: { cbn. unfold triggerUB. my_steps. }
+      my_steps.
+      unfold Mem.store in *. des_ifs_safe.
+      assert(U: Mem.cnts m0 blk ofs = Some v).
+      { destruct blk; ss; et. rewrite <- BLK; et. }
+      des_ifs. my_steps.
+      rr. esplits; ss; et.
+      rr. ss. esplits; try lia.
+      - ii. extensionalities ofs0. rewrite BLK; ss.
+      - ii. des_ifs; ss; et.
+    }
+    {
+      esplits; ss; eauto 10. ii. des; subst.
+      assert(W:=extends_valid_ptr SIMMRS1).
+      rr in SIMMRS1. des.
+      eapply sim_itree_fsubset with []; ss.
+      unfold cfunU, cmpF.
+      ginit. my_steps.
+      destruct (Any.downcast y) eqn:T.
+      2: { cbn. unfold triggerUB. my_steps. }
+      my_steps. des_ifs; my_steps; unfold triggerUB; my_steps.
+      destruct (vcmp m1 v v0) eqn:U.
+      2: { cbn. unfold triggerUB. my_steps. }
+      unfold vcmp in *. des_ifs; my_steps; des_ifs; my_steps; rr; esplits; ss;
+        bsimpl; des; des_sumbool; ss; subst; exploit W; et; i; try congruence.
+      - clear Heq2. exploit W; et; i; try congruence.
+      - clear Heq2. exploit W; et; i; try congruence.
+    }
+  Qed.
+
 End PROOF.
